lower use of `pure`, following advice from @nikswamy

pulse/examples/steel/LListWithTail.fst
@@ -73,6 +73,20 @@ let pure_star_interp (p:slprop u#a) (q:prop) (m:mem)
   pure_star_interp p q m;
   emp_unit p
 
+let pure_cut
+  (p: slprop)
+  (q: prop)
+  (f: (m: mem) -> Lemma (requires (interp p m)) (ensures q))
+: Steel unit
+    p
+    (fun _ -> p)
+    (requires (fun _ -> True))
+    (ensures (fun _ _ _ -> q))
+=
+  change_slprop p (p `star` pure q) (fun m -> f m; pure_star_interp p q m);
+  let _ : squash q = elim_pure q in
+  noop ()
+
 val intro_llist_nil (a:Type)
    : SteelT unit emp (fun _ -> llist_with_tail (null_llist #a) [])
 
@@ -90,15 +104,14 @@ val intro_llist_cons_nil'
   (m: mem)
 : Lemma
   (requires (
-    interp (pts_to ptr.head full_perm x `star` pure (is_null (LL.next x) == true) `star` pure (ptr.tail == ptr.head)) m
+    is_null (LL.next x) == true /\ ptr.tail == ptr.head /\
+    interp (pts_to ptr.head full_perm x) m
   ))
   (ensures (interp (llist_with_tail ptr [x]) m))
 
 let intro_llist_cons_nil'
   a ptr x m
 =
-  pure_star_interp (pts_to ptr.head full_perm x `star` pure (is_null (LL.next x) == true)) (ptr.tail == ptr.head) m;
-  pure_star_interp (pts_to ptr.head full_perm x) (is_null (LL.next x) == true) m;
   norm_spec [delta; zeta] (llist_with_tail ptr [x]);
   pure_star_interp (llist_with_tail_fragment ptr x []) (is_null (LL.next (L.last [x])) == true) m;
   norm_spec [delta; zeta] (llist_with_tail_fragment ptr x []);
@@ -108,22 +121,26 @@ let intro_llist_cons_nil
   (a: Type)
   (ptr: t a)
   (x: LL.cell a)
-: SteelT unit
-    (pts_to ptr.head full_perm x `star` pure (is_null (LL.next x) == true) `star` pure (ptr.tail == ptr.head))
+: Steel unit
+    (pts_to ptr.head full_perm x)
     (fun _ -> llist_with_tail ptr [x])
+    (requires (fun _ -> is_null (LL.next x) == true /\ ptr.tail == ptr.head))
+    (ensures (fun _ _ _ -> True))
 =
   change_slprop
-    (pts_to ptr.head full_perm x `star` pure (is_null (LL.next x) == true) `star` pure (ptr.tail == ptr.head))
+    (pts_to ptr.head full_perm x)
     (llist_with_tail ptr [x])
     (fun m -> intro_llist_cons_nil' a ptr x m)
 
 val push_nil
   (a: Type)
   (x: a)
-: SteelT
+: Steel
     (t a & Ghost.erased (list (LL.cell a)))
     (emp)
-    (fun z -> llist_with_tail (fst z) (snd z) `star` pure (LL.datas (snd z) == [x]))
+    (fun z -> llist_with_tail (fst z) (snd z))
+    (requires (fun _ -> True))
+    (ensures (fun _ z _ -> LL.datas (snd z) == [x]))
 
 #push-options "--ide_id_info_off"
 
@@ -133,8 +150,6 @@ let push_nil
   let x = LL.mk_cell null e in
   let px = alloc x in
   let ptr = {head = px ; tail = px} in
-  intro_pure (is_null (LL.next x) == true);
-  intro_pure (ptr.tail == ptr.head);
   change_slprop
     (pts_to px full_perm x)
     (pts_to ptr.head full_perm x)
@@ -145,7 +160,6 @@ let push_nil
     (llist_with_tail ptr [x])
     (llist_with_tail (fst z) (snd z))
     (fun _ -> ());
-  intro_pure (LL.datas (Ghost.reveal (snd z)) == [e]);
   z
 
 let pts_to_not_null_intro
@@ -153,12 +167,12 @@ let pts_to_not_null_intro
   (x:ref a)
   (p:perm)
   (v: Ghost.erased a)
-: SteelT unit (pts_to x p v) (fun _ -> pts_to x p v `star` pure (is_null x == false))
+: Steel unit (pts_to x p v) (fun _ -> pts_to x p v)
+  (requires (fun _ -> True))
+  (ensures (fun _ _ _ -> is_null x == false))
 =
-  change_slprop  (pts_to x p v) (pts_to x p v `star` pure (is_null x == false))
-  (fun m ->
-    pts_to_not_null x p v m;
-    pure_star_interp (pts_to x p v) (is_null x == false) m
+  pure_cut (pts_to x p v) (is_null x == false) (fun m ->
+    pts_to_not_null x p v m
   )
 
 let llist_is_nil_intro
@@ -186,18 +200,19 @@ val llist_is_nil
   (a: Type)
   (ptr: t a)
   (l: Ghost.erased (list (LL.cell a)))
-: SteelT
+: Steel
     bool
     (llist_with_tail ptr l)
-    (fun b -> llist_with_tail ptr l `star` pure (Nil? l == b))
+    (fun _ -> llist_with_tail ptr l)
+    (requires (fun _ -> True))
+    (ensures (fun _ b _ -> Nil? l == b))
 
 let llist_is_nil
   a ptr l
 =
   let res = (is_null ptr.head) in
-  change_slprop (llist_with_tail ptr l) (llist_with_tail ptr l `star` pure (Nil? l == res)) (fun m ->
-    llist_is_nil_intro a ptr l m;
-    pure_star_interp (llist_with_tail ptr l) (Nil? l == res) m
+  pure_cut (llist_with_tail ptr l) (Nil? l == res) (fun m ->
+    llist_is_nil_intro a ptr l m
   );
   res
 
@@ -210,8 +225,9 @@ val intro_llist_cons_cons'
   (m: mem)
 : Lemma
   (requires (interp
-    (llist_with_tail ptr0 q `star` pts_to ptr.head full_perm x `star` pure (ptr0.head == LL.next x) `star` pure (ptr0.tail == ptr.tail) `star` pure (Cons? q == true))
-    m
+    (llist_with_tail ptr0 q `star` pts_to ptr.head full_perm x)
+    m /\
+    ptr0.head == LL.next x /\ ptr0.tail == ptr.tail /\ Cons? q == true
   ))
   (ensures (interp
     (llist_with_tail ptr (x :: q))
@@ -221,18 +237,6 @@ let intro_llist_cons_cons'
   a ptr ptr0 x q m
 =
   (* destruct the hypothesis *)
-  pure_star_interp
-    (llist_with_tail ptr0 q `star` pts_to ptr.head full_perm x `star` pure (ptr0.head == LL.next x) `star` pure (ptr0.tail == ptr.tail))
-    (Cons? q == true)
-    m;
-  pure_star_interp
-    (llist_with_tail ptr0 q `star` pts_to ptr.head full_perm x `star` pure (ptr0.head == LL.next x))
-    (ptr0.tail == ptr.tail)
-    m;
-  pure_star_interp
-    (llist_with_tail ptr0 q `star` pts_to ptr.head full_perm x)
-    (ptr0.head == LL.next x)
-    m;
   star_commutative
     (llist_with_tail ptr0 q)
     (pts_to ptr.head full_perm x);
@@ -261,13 +265,15 @@ let intro_llist_cons_cons
   (ptr0 : t a)
   (x: LL.cell a)
   (q: Ghost.erased (list (LL.cell a)))
-: SteelT
+: Steel
     unit
-    (llist_with_tail ptr0 q `star` pts_to ptr.head full_perm x `star` pure (ptr0.head == LL.next x) `star` pure (ptr0.tail == ptr.tail) `star` pure (Cons? q == true))
+    (llist_with_tail ptr0 q `star` pts_to ptr.head full_perm x)
     (fun _ -> llist_with_tail ptr (x :: q))
+    (requires (fun _ -> ptr0.head == LL.next x /\ ptr0.tail == ptr.tail /\ Cons? q == true))
+    (ensures (fun _ _ _ -> True))
 =
   change_slprop
-    (llist_with_tail ptr0 q `star` pts_to ptr.head full_perm x `star` pure (ptr0.head == LL.next x) `star` pure (ptr0.tail == ptr.tail) `star` pure (Cons? q == true))
+    (llist_with_tail ptr0 q `star` pts_to ptr.head full_perm x)
     (llist_with_tail ptr (x :: q))
     (fun m -> intro_llist_cons_cons' a ptr ptr0 x q m)
 
@@ -276,10 +282,12 @@ val push_cons
   (ptr: t a)
   (x: a)
   (q: Ghost.erased (list (LL.cell a)))
-: SteelT
+: Steel
     (t a & Ghost.erased (list (LL.cell a)))
-    (llist_with_tail ptr q `star` pure (Cons? q == true))
-    (fun z -> llist_with_tail (fst z) (snd z) `star` pure (LL.datas (snd z) == x :: LL.datas q))
+    (llist_with_tail ptr q)
+    (fun z -> llist_with_tail (fst z) (snd z))
+    (requires (fun _ -> Cons? q == true))
+    (ensures (fun _ z _ -> LL.datas (snd z) == x :: LL.datas q))
 
 let push_cons
   a ptr0 e q
@@ -291,15 +299,12 @@ let push_cons
     (pts_to px full_perm x)
     (pts_to ptr.head full_perm x)
     (fun _ -> ());
-  intro_pure (ptr0.head == LL.next x);
-  intro_pure (ptr0.tail == ptr.tail);
   intro_llist_cons_cons a ptr ptr0 x q;
   let z = (ptr, Ghost.hide (x :: q)) in
   change_slprop
     (llist_with_tail ptr (Ghost.hide (x :: q)))
     (llist_with_tail (fst z) (snd z))
     (fun _ -> ());
-  intro_pure (LL.datas (Ghost.reveal (snd z)) == e :: LL.datas q);
   z
 
 val push
@@ -307,26 +312,23 @@ val push
   (ptr: t a)
   (x: a)
   (q: Ghost.erased (list (LL.cell a)))
-: SteelT
+: Steel
     (t a & Ghost.erased (list (LL.cell a)))
     (llist_with_tail ptr q)
-    (fun z -> llist_with_tail (fst z) (snd z) `star` pure (LL.datas (snd z) == x :: LL.datas q))
+    (fun z -> llist_with_tail (fst z) (snd z))
+    (requires (fun _ -> True))
+    (ensures (fun _ z _ -> LL.datas (snd z) == x :: LL.datas q))
 
 let push
   a ptr x q
 =
   let is_nil = llist_is_nil a ptr q in
-  elim_pure (Nil? q == is_nil);
   if is_nil
   then begin
     drop (llist_with_tail ptr q);
-    let res = push_nil a x in
-    elim_pure (LL.datas (Ghost.reveal (snd res)) == [x]);
-    intro_pure (LL.datas (snd res) == x :: LL.datas q);
-    res
+    push_nil a x
   end
   else begin
-    intro_pure (Cons? q == true);
-    let res = push_cons a ptr x q in
-    res
+    noop (); // FIXME: WHY WHY WHY? (Alternatively, let res = push_cons ... in res will also work, but still, WHY?)
+    push_cons a ptr x q
   end
